mathcomp_compat.v
@@ -1,0 +1,79 @@
+(** We define these instances in their own file to avoid conflicts between
+mathcomp and stdpp definitions. *)
+
+From mathcomp Require Import all_ssreflect.
+From deriving Require Import deriving.
+From stdpp Require base countable.
+Require Import Coq.ZArith.ZArith.
+Require Import Permutation.
+From iris.heap_lang Require locations.
+
+(* FIXME: This should exist in deriving *)
+Definition positive_orderMixin :=
+  [derive orderMixin for positive].
+Canonical positive_porderType :=
+  Eval hnf in POrderType tt positive positive_orderMixin.
+Canonical positive_latticeType :=
+  Eval hnf in LatticeType positive positive_orderMixin.
+Canonical positive_distrLatticeType :=
+  Eval hnf in DistrLatticeType positive positive_orderMixin.
+Canonical positive_orderType :=
+  Eval hnf in OrderType positive positive_orderMixin.
+
+Definition Z_orderMixin :=
+  [derive orderMixin for Z].
+Canonical Z_porderType :=
+  Eval hnf in POrderType tt Z Z_orderMixin.
+Canonical Z_latticeType :=
+  Eval hnf in LatticeType Z Z_orderMixin.
+Canonical Z_distrLatticeType :=
+  Eval hnf in DistrLatticeType Z Z_orderMixin.
+Canonical Z_orderType :=
+  Eval hnf in OrderType Z Z_orderMixin.
+
+Canonical loc_newType := [newType for locations.loc_car].
+Definition loc_eqMixin := [eqMixin of locations.loc by <:].
+Canonical loc_eqType := EqType locations.loc loc_eqMixin.
+Definition loc_choiceMixin := [choiceMixin of locations.loc by <:].
+Canonical loc_choiceType := Eval hnf in ChoiceType locations.loc loc_choiceMixin.
+Definition loc_countMixin := [countMixin of locations.loc by <:].
+Canonical loc_countType := Eval hnf in CountType locations.loc loc_countMixin.
+Definition loc_porderMixin := [porderMixin of locations.loc by <:].
+Canonical loc_porderType :=
+  Eval hnf in POrderType tt locations.loc loc_porderMixin.
+Definition loc_orderMixin := [totalOrderMixin of locations.loc by <:].
+Canonical loc_latticeType :=
+  Eval hnf in LatticeType locations.loc loc_orderMixin.
+Canonical loc_distrLatticeType :=
+  Eval hnf in DistrLatticeType locations.loc loc_orderMixin.
+Canonical loc_orderType :=
+  Eval hnf in OrderType locations.loc loc_orderMixin.
+
+Definition def_eq_decision (T : eqType) : base.RelDecision (@eq T) :=
+  fun x y => Bool.reflect_dec _ _ (x =P y).
+
+Definition def_countable (T : countType) (H : base.RelDecision (@eq T)) : countable.Countable T.
+Proof.
+apply:
+  (@countable.inj_countable _ _ countable.nat_countable T H pickle unpickle).
+exact: pickleK.
+Qed.
+
+Lemma perm_Permutation (T : eqType) (s1 s2 : seq T) :
+  reflect (Permutation s1 s2) (perm_eq s1 s2).
+Proof.
+apply/(iffP idP).
+  rewrite perm_sym; elim: s1 s2 => [_ /perm_nilP -> //|x s1 IH] s2 ps1s2.
+  have x_s2 : x \in s2 by rewrite (perm_mem ps1s2) inE eqxx.
+  case/path.splitP: x_s2 ps1s2 => s21 s22 ps1s2.
+  have {}ps1s2: perm_eq (s21 ++ s22) s1.
+    by move: ps1s2; rewrite -cats1 perm_catAC perm_catC /= perm_cons.
+  rewrite -cats1 -catA /=.
+  by apply: Permutation_cons_app; apply: IH.
+elim: s1 s2 / => //.
+- by move=> x s1 s2 _ IH; rewrite perm_cons.
+- move=> x1 x2 s.
+  rewrite (perm_cat2r s [:: x2; x1] [:: x1; x2]) /=.
+  by rewrite -cat1s -[[:: x1; x2]]cat1s perm_catC.
+- by move=> ? ? ? _ ? _; apply: seq.perm_trans.
+Qed.
