pre_term.v
@@ -1,0 +1,459 @@
+From mathcomp Require Import all_ssreflect.
+From deriving Require Import deriving.
+From crypto Require Import mathcomp_compat lib.
+Require Import Coq.ZArith.ZArith.
+From iris.heap_lang Require Import locations.
+
+Import Order.POrderTheory Order.TotalTheory.
+
+Inductive key_type := Enc | Dec.
+
+Canonical key_type_indDef := [indDef for key_type_rect].
+Canonical key_type_indType := IndType key_type key_type_indDef.
+Definition key_type_eqMixin := [derive eqMixin for key_type].
+Canonical key_type_eqType := EqType key_type key_type_eqMixin.
+Definition key_type_choiceMixin := [derive choiceMixin for key_type].
+Canonical key_type_choiceType :=
+  Eval hnf in ChoiceType key_type key_type_choiceMixin.
+Definition key_type_countMixin := [derive countMixin for key_type].
+Canonical key_type_countType :=
+  Eval hnf in CountType key_type key_type_countMixin.
+Definition key_type_orderMixin :=
+  [derive orderMixin for key_type].
+Canonical key_type_porderType :=
+  Eval hnf in POrderType tt key_type key_type_orderMixin.
+Canonical key_type_latticeType :=
+  Eval hnf in LatticeType key_type key_type_orderMixin.
+Canonical key_type_distrLatticeType :=
+  Eval hnf in DistrLatticeType key_type key_type_orderMixin.
+Canonical key_type_orderType :=
+  Eval hnf in OrderType key_type key_type_orderMixin.
+
+Module PreTerm.
+
+Unset Elimination Schemes.
+Inductive pre_term :=
+| PTInt of Z
+| PTPair of pre_term & pre_term
+| PTNonce of loc
+| PTKey of key_type & pre_term
+| PTEnc of pre_term & pre_term
+| PTHash of pre_term
+| PTExp of pre_term & list pre_term.
+Set Elimination Schemes.
+
+Definition pre_term_rect'
+  (T1 : pre_term -> Type)
+  (T2 : list pre_term -> Type)
+  (H1 : forall n, T1 (PTInt n))
+  (H2 : forall t1, T1 t1 -> forall t2, T1 t2 -> T1 (PTPair t1 t2))
+  (H3 : forall l, T1 (PTNonce l))
+  (H4 : forall kt t, T1 t -> T1 (PTKey kt t))
+  (H5 : forall t1, T1 t1 -> forall t2, T1 t2 -> T1 (PTEnc t1 t2))
+  (H6 : forall t, T1 t -> T1 (PTHash t))
+  (H7 : forall t, T1 t -> forall ts, T2 ts -> T1 (PTExp t ts))
+  (H8 : T2 [::])
+  (H9 : forall t, T1 t -> forall ts, T2 ts -> T2 (t :: ts)) :=
+  fix loop1 t {struct t} : T1 t :=
+    match t with
+    | PTInt n => H1 n
+    | PTPair t1 t2 => H2 t1 (loop1 t1) t2 (loop1 t2)
+    | PTNonce l => H3 l
+    | PTKey kt t => H4 kt t (loop1 t)
+    | PTEnc t1 t2 => H5 t1 (loop1 t1) t2 (loop1 t2)
+    | PTHash t => H6 t (loop1 t)
+    | PTExp t ts =>
+      let fix loop2 ts {struct ts} : T2 ts :=
+          match ts with
+          | [::] => H8
+          | t :: ts => H9 t (loop1 t) ts (loop2 ts)
+          end in
+      H7 t (loop1 t) ts (loop2 ts)
+    end.
+
+Definition list_pre_term_rect'
+  (T1 : pre_term -> Type)
+  (T2 : list pre_term -> Type)
+  (H1 : forall n, T1 (PTInt n))
+  (H2 : forall t1, T1 t1 -> forall t2, T1 t2 -> T1 (PTPair t1 t2))
+  (H3 : forall l, T1 (PTNonce l))
+  (H4 : forall kt t, T1 t -> T1 (PTKey kt t))
+  (H5 : forall t1, T1 t1 -> forall t2, T1 t2 -> T1 (PTEnc t1 t2))
+  (H6 : forall t, T1 t -> T1 (PTHash t))
+  (H7 : forall t, T1 t -> forall ts, T2 ts -> T1 (PTExp t ts))
+  (H8 : T2 [::])
+  (H9 : forall t, T1 t -> forall ts, T2 ts -> T2 (t :: ts)) :=
+  fix loop2 ts {struct ts} : T2 ts :=
+    match ts with
+    | [::] => H8
+    | t :: ts =>
+      H9 t (pre_term_rect' T1 T2 H1 H2 H3 H4 H5 H6 H7 H8 H9 t) ts (loop2 ts)
+    end.
+
+Combined Scheme pre_term_list_pre_term_rect
+  from pre_term_rect', list_pre_term_rect'.
+
+Definition pre_term_list_pre_term_indDef :=
+  [indDef for pre_term_list_pre_term_rect].
+Canonical pre_term_indType := IndType pre_term pre_term_list_pre_term_indDef.
+Definition pre_term_eqMixin :=
+  [derive eqMixin for pre_term].
+Canonical pre_term_eqType :=
+  Eval hnf in EqType pre_term pre_term_eqMixin.
+Definition pre_term_choiceMixin :=
+  [derive choiceMixin for pre_term].
+Canonical pre_term_choiceType :=
+  Eval hnf in ChoiceType pre_term pre_term_choiceMixin.
+Definition pre_term_countMixin :=
+  [derive countMixin for pre_term].
+Canonical pre_term_countType :=
+  Eval hnf in CountType pre_term pre_term_countMixin.
+Definition pre_term_orderMixin :=
+  [derive orderMixin for pre_term].
+Canonical pre_term_porderType :=
+  Eval hnf in POrderType tt pre_term pre_term_orderMixin.
+Canonical pre_term_latticeType :=
+  Eval hnf in LatticeType pre_term pre_term_orderMixin.
+Canonical pre_term_distrLatticeType :=
+  Eval hnf in DistrLatticeType pre_term pre_term_orderMixin.
+Canonical pre_term_orderType :=
+  Eval hnf in OrderType pre_term pre_term_orderMixin.
+
+Definition pre_term_rect (T : pre_term -> Type)
+  (H1 : forall n, T (PTInt n))
+  (H2 : forall t1, T t1 -> forall t2, T t2 -> T (PTPair t1 t2))
+  (H3 : forall l, T (PTNonce l))
+  (H4 : forall kt t, T t -> T (PTKey kt t))
+  (H5 : forall t1, T t1 -> forall t2, T t2 -> T (PTEnc t1 t2))
+  (H6 : forall t, T t -> T (PTHash t))
+  (H7 : forall t, T t ->
+        forall ts, foldr (fun t R => T t * R)%type unit ts ->
+          T (PTExp t ts)) t : T t.
+Proof.
+exact: (@pre_term_rect' T (foldr (fun t R => T t * R)%type unit)).
+Defined.
+
+Definition pre_term_ind (T : pre_term -> Prop) :=
+  @pre_term_rect T.
+
+Fixpoint height pt :=
+  match pt with
+  | PTInt _ => 1
+  | PTPair t1 t2 => S (maxn (height t1) (height t2))
+  | PTNonce _ => 1
+  | PTKey _ t => S (height t)
+  | PTEnc k t => S (maxn (height k) (height t))
+  | PTHash t => S (height t)
+  | PTExp t ts => S (\max_(x <- height t :: map height ts) x)
+  end.
+
+Definition is_exp pt := if pt is PTExp _ _ then true else false.
+
+Definition exp pt pts :=
+  match pt with
+  | PTExp pt pts' => PTExp pt (sort <=%O (pts' ++ pts))
+  | _ => PTExp pt (sort <=%O pts)
+  end.
+
+Variant exp_spec pt pts : pre_term -> Type :=
+| PTExpExp pt' pts' of pt = PTExp pt' pts'
+: exp_spec pt pts (PTExp pt' (sort <=%O (pts' ++ pts)))
+
+| PTExpNExp of exp pt pts = PTExp pt (sort <=%O pts)
+& ~~ is_exp pt
+: exp_spec pt pts (PTExp pt (sort <=%O pts)).
+
+Lemma expP pt pts : exp_spec pt pts (exp pt pts).
+Proof. by case: pt=> /= *; constructor. Qed.
+
+(* An alternative of the above that avoids relying on mathcomp definitions *)
+Variant exp_spec' pt pts : pre_term -> Type :=
+| PTExpExp' pt' pts' pts'' of pt = PTExp pt' pts'
+& Permutation.Permutation pts'' (List.app pts' pts)
+: exp_spec' pt pts (PTExp pt' pts'')
+
+| PTExpNExp' pts' of exp pt pts = PTExp pt pts'
+& Permutation.Permutation pts' pts
+: exp_spec' pt pts (PTExp pt pts').
+
+Lemma expP' pt pts : exp_spec' pt pts (exp pt pts).
+Proof.
+by case: expP=> [? ? ->|? ?]; [eleft|eright]; eauto;
+apply/perm_Permutation; rewrite perm_sort.
+Qed.
+
+Fixpoint normalize pt :=
+  match pt with
+  | PTInt n => PTInt n
+  | PTPair t1 t2 => PTPair (normalize t1) (normalize t2)
+  | PTNonce a => PTNonce a
+  | PTKey kt t => PTKey kt (normalize t)
+  | PTEnc k t => PTEnc (normalize k) (normalize t)
+  | PTHash t => PTHash (normalize t)
+  | PTExp t ts =>
+    let t  := normalize t in
+    let ts := [seq normalize t | t <- ts] in
+    exp t ts
+  end.
+
+Fixpoint wf_term pt :=
+  match pt with
+  | PTInt _ => true
+  | PTPair pt1 pt2 => wf_term pt1 && wf_term pt2
+  | PTNonce _ => true
+  | PTKey _ pt => wf_term pt
+  | PTEnc k pt => wf_term k && wf_term pt
+  | PTHash pt => wf_term pt
+  | PTExp pt pts =>
+    [&& ~~ is_exp pt, wf_term pt, all wf_term pts & sorted <=%O pts]
+  end.
+
+Lemma wf_exp pt pts : wf_term pt -> all wf_term pts -> wf_term (exp pt pts).
+Proof.
+case: expP => [pt' pts' ->|] /=.
+- case/and4P=> -> -> norm_pts' _ /=.
+  by rewrite all_sort all_cat norm_pts' /= sort_le_sorted => ->.
+- by move=> _ -> -> /=; rewrite sort_le_sorted andbT all_sort.
+Qed.
+
+Lemma wf_normalize pt : wf_term (normalize pt).
+Proof.
+move: {2}(height pt) (leqnn (height pt)) => n.
+elim: n pt => [[] //|n IH]; case=> //=.
+- by move=> pt1 pt2; rewrite ltnS geq_max; case/andP=> /IH -> /IH ->.
+- by move=> pt1 pt2; rewrite ltnS geq_max; case/andP=> /IH -> /IH ->.
+move=> pt pts; rewrite ltnS big_cons geq_max big_map_id big_tnth.
+case/andP => /IH e_pt /bigmax_leqP e_pts; rewrite wf_exp //.
+rewrite all_map -[pts]in_tupleE; apply/allP => pt' /tnthP [] ? ->.
+apply: IH; exact: e_pts.
+Qed.
+
+Lemma normalize_wf pt : wf_term pt -> normalize pt = pt.
+Proof.
+move: {2}(height pt) (leqnn (height pt)) => n.
+elim: n pt => [[] //|n IH]; case=> //=.
+- move=> pt1 pt2; rewrite ltnS geq_max.
+  case/andP=> pt1_n pt2_n; case/andP=> norm_pt1 norm_pt2.
+  by rewrite !IH.
+- by move=> kt p; rewrite ltnS => ? ?; rewrite IH.
+- move=> pt1 pt2; rewrite ltnS geq_max.
+  case/andP=> pt1_n pt2_n; case/andP=> norm_pt1 norm_pt2.
+  by rewrite !IH.
+- by move=> p; rewrite ltnS => ? ?; rewrite IH.
+move=> pt pts; rewrite ltnS big_cons geq_max big_map_id big_tnth.
+case/andP => /IH e_pt /bigmax_leqP e_pts.
+have {}e_pts pt': pt' \in in_tuple pts -> wf_term pt' -> normalize pt' = pt'.
+  by case/tnthP=> ? ->; apply: IH; apply: e_pts.
+case/and4P=> nexp norm_pt /allP norm_pts sort_pts.
+rewrite e_pt // map_id_in; last first.
+  by move=> ? in_pts; apply: e_pts (in_pts) _; apply: norm_pts.
+by case: expP nexp=> [pt' pts' -> //|_ _ _]; rewrite sort_le_id.
+Qed.
+
+Lemma normalize_idem pt : normalize (normalize pt) = normalize pt.
+Proof. apply: normalize_wf; exact: wf_normalize. Qed.
+
+End PreTerm.
+
+Canonical PreTerm.pre_term_eqType.
+Canonical PreTerm.pre_term_choiceType.
+Canonical PreTerm.pre_term_countType.
+Canonical PreTerm.pre_term_porderType.
+Canonical PreTerm.pre_term_latticeType.
+Canonical PreTerm.pre_term_distrLatticeType.
+Canonical PreTerm.pre_term_orderType.
+
+Record term := Term_ {
+  val_term : PreTerm.pre_term;
+  _ : PreTerm.wf_term val_term;
+}.
+
+Canonical term_subType := [subType for val_term].
+Definition term_eqMixin := [eqMixin of term by <:].
+Canonical term_eqType := EqType term term_eqMixin.
+Definition term_choiceMixin := [choiceMixin of term by <:].
+Canonical term_choiceType := Eval hnf in ChoiceType term term_choiceMixin.
+Definition term_countMixin := [countMixin of term by <:].
+Canonical term_countType := Eval hnf in CountType term term_countMixin.
+Definition term_porderMixin := [porderMixin of term by <:].
+Canonical term_porderType :=
+  Eval hnf in POrderType tt term term_porderMixin.
+Definition term_orderMixin := [totalOrderMixin of term by <:].
+Canonical term_latticeType :=
+  Eval hnf in LatticeType term term_orderMixin.
+Canonical term_distrLatticeType :=
+  Eval hnf in DistrLatticeType term term_orderMixin.
+Canonical term_orderType :=
+  Eval hnf in OrderType term term_orderMixin.
+
+Fact Term_key : unit. Proof. exact: tt. Qed.
+Definition Term :=
+  locked_with Term_key (
+    fun t => @Term_ (PreTerm.normalize t) (PreTerm.wf_normalize t)
+  ).
+Canonical Term_unlockable := [unlockable of Term].
+
+Implicit Types (t k : term) (ts : seq term).
+
+Definition TInt n := Term (PreTerm.PTInt n).
+Definition TPair t1 t2 := Term (PreTerm.PTPair (val t1) (val t2)).
+Definition TNonce a := Term (PreTerm.PTNonce a).
+Definition TKey kt t := Term (PreTerm.PTKey kt (val t)).
+Definition TEnc k t := Term (PreTerm.PTEnc (val k) (val t)).
+Definition THash t := Term (PreTerm.PTHash (val t)).
+Definition TExp t ts := Term (PreTerm.PTExp (val t) [seq val t | t <- ts]).
+
+Lemma val_termK : cancel val_term Term.
+Proof.
+case/SubP=> pt wf_pt; rewrite unlock; apply: val_inj.
+exact: PreTerm.normalize_wf.
+Qed.
+
+Lemma val_term_TInt n : val_term (TInt n) = PreTerm.PTInt n.
+Proof. by rewrite /TInt unlock. Qed.
+
+Lemma val_term_TPair t1 t2 :
+  val_term (TPair t1 t2) = PreTerm.PTPair (val_term t1) (val_term t2).
+Proof. by rewrite /TPair unlock /= !PreTerm.normalize_wf ?valP. Qed.
+
+Lemma val_term_TNonce a : val_term (TNonce a) = PreTerm.PTNonce a.
+Proof. by rewrite /TNonce unlock. Qed.
+
+Lemma val_term_TKey kt t : val_term (TKey kt t) = PreTerm.PTKey kt (val_term t).
+Proof. by rewrite /TKey unlock /= PreTerm.normalize_wf ?valP. Qed.
+
+Lemma val_term_TEnc k t :
+  val_term (TEnc k t) = PreTerm.PTEnc (val_term k) (val_term t).
+Proof. by rewrite /TEnc unlock /= !PreTerm.normalize_wf ?valP. Qed.
+
+Lemma val_term_THash t :
+  val_term (THash t) = PreTerm.PTHash (val_term t).
+Proof. by rewrite /THash unlock /= !PreTerm.normalize_wf ?valP. Qed.
+
+Lemma normalize_terms ts :
+  map PreTerm.normalize (map val_term ts) = map val_term ts.
+Proof.
+rewrite map_id_in // => _ /mapP [] {}t t_ts ->.
+apply: PreTerm.normalize_wf; apply: valP.
+Qed.
+
+Lemma val_term_TExp t ts :
+  val_term (TExp t ts) = PreTerm.exp (val_term t) (List.map val_term ts).
+Proof.
+by rewrite /TExp unlock /= PreTerm.normalize_wf ?valP // normalize_terms.
+Qed.
+
+Definition val_termE :=
+  (val_term_TInt,
+   val_term_TPair,
+   val_term_TNonce,
+   val_term_TKey,
+   val_term_TEnc,
+   val_term_THash,
+   val_term_TExp).
+
+Lemma Term_PTInt n : Term (PreTerm.PTInt n) = TInt n.
+Proof. by []. Qed.
+
+Lemma Term_PTPair pt1 pt2 :
+  Term (PreTerm.PTPair pt1 pt2) = TPair (Term pt1) (Term pt2).
+Proof.
+by apply: val_inj; rewrite /TPair unlock /= !PreTerm.normalize_idem.
+Qed.
+
+Lemma Term_PTNonce a : Term (PreTerm.PTNonce a) = TNonce a.
+Proof. by []. Qed.
+
+Lemma Term_PTKey kt pt : Term (PreTerm.PTKey kt pt) = TKey kt (Term pt).
+Proof.
+by apply: val_inj; rewrite /TKey unlock /= !PreTerm.normalize_idem.
+Qed.
+
+Lemma Term_PTEnc pt1 pt2 :
+  Term (PreTerm.PTEnc pt1 pt2) = TEnc (Term pt1) (Term pt2).
+Proof.
+by apply: val_inj; rewrite /TEnc unlock /= !PreTerm.normalize_idem.
+Qed.
+
+Lemma Term_PTHash pt : Term (PreTerm.PTHash pt) = THash (Term pt).
+Proof.
+by apply: val_inj; rewrite /THash unlock /= !PreTerm.normalize_idem.
+Qed.
+
+Lemma Term_PTExp pt pts :
+  Term (PreTerm.PTExp pt pts) = TExp (Term pt) (map Term pts).
+Proof.
+apply: val_inj; rewrite /TExp unlock /= PreTerm.normalize_idem.
+by rewrite normalize_terms -map_comp.
+Qed.
+
+Definition TermE :=
+  (Term_PTInt,
+   Term_PTPair,
+   Term_PTNonce,
+   Term_PTKey,
+   Term_PTEnc,
+   Term_PTHash,
+   Term_PTExp).
+
+Lemma perm_sort_leP d (T : orderType d) (s1 s2 : seq T) :
+  reflect (sort <=%O s1 = sort <=%O s2) (perm_eq s1 s2).
+Proof.
+apply/perm_sortP; by [apply: le_total|apply: le_trans|apply: le_anti].
+Qed.
+
+Lemma TExpA t ts1 ts2 : TExp (TExp t ts1) ts2 = TExp t (ts1 ++ ts2)%list.
+Proof.
+apply: val_inj => /=; rewrite !val_termE -[List.map]/@map map_cat.
+case: (PreTerm.expP (val_term t)) => [pt' pts' e_t|_ nexp] /=.
+  rewrite e_t /=; congr PreTerm.PTExp.
+  by apply/perm_sort_leP; rewrite catA perm_cat2r perm_sort.
+case: PreTerm.expP nexp => [? ? -> //|_ _ _].
+by congr PreTerm.PTExp; apply/perm_sort_leP; rewrite perm_cat2r perm_sort.
+Qed.
+
+Lemma TExp_perm t ts1 ts2 : perm_eq ts1 ts2 -> TExp t ts1 = TExp t ts2.
+Proof.
+move=> perm_ts12; apply: val_inj => /=.
+rewrite !val_termE -[List.map]/@map.
+case: PreTerm.expP => [pt' pts' ->|_ nexp] /=.
+  by congr PreTerm.PTExp; apply/perm_sort_leP; rewrite perm_cat2l perm_map.
+case: PreTerm.expP nexp => [? ? -> //|_ _ _].
+by congr PreTerm.PTExp; apply/perm_sort_leP; rewrite perm_map.
+Qed.
+
+Definition is_exp t := PreTerm.is_exp (val_term t).
+
+Lemma term_rect (T : term -> Type)
+  (H1 : forall n, T (TInt n))
+  (H2 : forall t1, T t1 ->
+        forall t2, T t2 ->
+        T (TPair t1 t2))
+  (H3 : forall a, T (TNonce a))
+  (H4 : forall kt t, T t -> T (TKey kt t))
+  (H5 : forall k, T k -> forall t, T t -> T (TEnc k t))
+  (H6 : forall t, T t -> T (THash t))
+  (H7 : forall t, T t -> ~~ is_exp t ->
+        forall ts, foldr (fun t R => T t * R)%type unit ts ->
+                   sorted <=%O ts ->
+        T (TExp t ts)) :
+  forall t, T t.
+Proof.
+move=> t; move: (valP t); rewrite -{2}[t]val_termK /=.
+elim: (val_term t) => {t};
+do ?by move=> *; rewrite /= TermE; eauto.
+- by move=> t1 IH1 t2 IH2 /= /andP [] ??; rewrite TermE; eauto.
+- by move=> t1 IH1 t2 IH2 /= /andP [] ??; rewrite TermE; eauto.
+move=> t IHt ts IHts; rewrite TermE /=.
+case/and4P=> nexp wf_t wf_ts sorted_ts; apply: H7; eauto.
+- by rewrite /is_exp unlock /= PreTerm.normalize_wf.
+- elim: ts IHts wf_ts {sorted_ts} => //= {IHt nexp wf_t}t ts IH [??].
+  by case/andP=> wf_t wf_ts; split; eauto.
+have e_ts: ts = map val_term (map Term ts).
+  rewrite -map_comp map_id_in // => t' t'_ts.
+  rewrite unlock /= PreTerm.normalize_wf //.
+  exact: (allP wf_ts).
+by rewrite e_ts sorted_map in sorted_ts.
+Qed.
+
+Definition term_ind (P : term -> Prop) := @term_rect P.
